src/TV/mtv_correct.v
@@ -1,0 +1,96 @@
+Add LoadPath "../ssa/ott".
+Add LoadPath "../ssa/monads".
+Add LoadPath "../ssa".
+Add LoadPath "../ssa/compcert".
+Add LoadPath "../../../theory/metatheory_8.3".
+Require Import ssa_def.
+Require Import ssa_lib.
+Require Import List.
+Require Import targetdata.
+Require Import monad.
+Require Import Arith.
+Require Import ZArith.
+Require Import Metatheory.
+Require Import Memory.
+Require Import Values.
+Require Import ssa_mem.
+Require Import trace.
+Require Import symexe_def.
+Require Import assoclist.
+Require Import ssa_props.
+Require Import sub_tv_dec.
+Require Import sub_tv_infer.
+Require Import sub_tv.
+Require Import Coq.Bool.Sumbool.
+Require Import symexe_tactic.
+
+Definition ptr_has_basebound TD M vb ve vp : bool :=
+match (GV2ptr TD (getPointerSize TD) vb, 
+       GV2ptr TD (getPointerSize TD) ve,
+       GV2ptr TD (getPointerSize TD) vp) with
+| (Some (Vptr bb ob), Some (Vptr be oe), Some (Vptr bp op)) =>
+  let '(lo,hi) := Memory.Mem.bounds M bp in
+  bzeq bb be && bzeq bb bp && 
+  bzeq (Integers.Int.unsigned 31 ob) lo && 
+  bzeq (Integers.Int.unsigned 31 oe) hi           
+| _ => false
+end.
+
+(* fs: function table
+ * lc: local variable mappings
+*)
+Fixpoint valid_metadata (TD:TargetData) (fs lc:GVMap) (M:mem) (md:metadata) 
+  : bool :=
+match md with
+| nil => true
+| (fid,lbl,nth,b,e,p,true)::md' =>
+    match (lookupAL _ lc b, lookupAL _ lc e, lookupAL _ lc p) with
+    | (Some vb, Some ve, Some vp) => ptr_has_basebound TD M vb ve vp
+    | (None, None, None) => true
+    | _ => false
+    end && valid_metadata TD fs lc M md'
+| (fid,lbl,nth,b,e,p,false)::md' => 
+    match (lookupAL _ lc b, lookupAL _ lc e, lookupAL _ lc p) with
+    | (Some vb, Some ve, Some vp) => 
+        match (lookupFdefViaGVFromFunTable fs vb,
+               lookupFdefViaGVFromFunTable fs ve,
+               lookupFdefViaGVFromFunTable fs vp) with
+        | (Some fid1, Some fid2, Some fid3) => eq_id fid1 fid2 && eq_id fid3 fid3
+        | _ => false
+        end        
+    | (None, None, None) => true
+    | _ => false
+    end && valid_metadata TD fs lc M md'
+end.
+
+Definition valid_memdata_db (TD:TargetData) (M:mem) := 
+  forall addrofp t p vaddrofb vaddrofe ps lc gl oresult M' vb ve vp fid
+    addrofb addrofe,
+  mload TD M addrofp (typ_pointer t) Align.One = Some vp ->
+  is_hashLoadBaseBound fid = true ->
+  callLib M fid (params2GVs TD 
+    (p::
+     (typ_pointer (typ_pointer (typ_int Size.Eight)),vaddrofb)::
+     (typ_pointer (typ_pointer (typ_int Size.Eight)),vaddrofe)::
+     ps) lc gl) = 
+    Some (oresult, M') ->
+  getOperandValue TD vaddrofb lc gl = Some addrofb ->
+  getOperandValue TD vaddrofe lc gl = Some addrofe ->
+  mload TD M' addrofb (typ_pointer (typ_int Size.Eight)) Align.One = Some vb ->
+  mload TD M' addrofe (typ_pointer (typ_int Size.Eight)) Align.One = Some ve ->
+  ptr_has_basebound TD M vb ve vp = true.
+
+  
+
+
+(*****************************)
+(*
+*** Local Variables: ***
+*** coq-prog-name: "coqtop" ***
+*** coq-prog-args: ("-emacs-U" "-I" "~/SVN/sol/vol/src/ssa/monads" "-I" "~/SVN/sol/vol/src/ssa/ott" "-I" "~/SVN/sol/vol/src/ssa/compcert" "-I" "~/SVN/sol/theory/metatheory_8.3") ***
+*** End: ***
+ *)
+
+
+
+
